TouhouFormal/ECL.lean
@@ -1,1 +1,4 @@
 import TouhouFormal.ECL.Profile
+import TouhouFormal.ECL.Loader
+import TouhouFormal.ECL.Call
+import TouhouFormal.ECL.Timeline
